refine+crefine: update proofs for asid_map addition
The Refine proof update touches all architectures and also generic
files, because it needs to change the interface for arch_state_relation:
it needs access to aobjs_of' on ARCH64 to reconstruct the
abstract asid_map from the contents of ASIDPool entries on the Haskell
side.

CRefine has a minimal update to avoid a name clash.

Signed-off-by: Gerwin Klein <gerwin.klein@proofcraft.systems>

proof/refine/ARM_HYP/ArchStateRelation.thy
@@ -175,8 +175,10 @@ definition ghost_relation_wrapper_2 ::
 (* inside Arch locale, we have no need for the wrapper *)
 lemmas ghost_relation_wrapper_def[simp] = ghost_relation_wrapper_2_def
 
-definition arch_state_relation :: "(arch_state \<times> ARM_HYP_H.kernel_state) set" where
-  "arch_state_relation \<equiv> {(s, s') .
+(* aobjs' argument unused on this architecture *)
+definition arch_state_relation ::
+  "(obj_ref \<rightharpoonup> arch_kernel_object) \<Rightarrow> (arch_state \<times> ARM_HYP_H.kernel_state) set" where
+  "arch_state_relation aobjs' \<equiv> {(s, s') .
          arm_asid_table s = armKSASIDTable s' o ucast
        \<and> arm_hwasid_table s = armKSHWASIDTable s'
        \<and> arm_next_asid s = armKSNextASID s'
