proof/refine/X64/ArchInit_R.thy
@@ -40,7 +40,7 @@ lemma ghost_relation_wrapper_arch_intermediate_state[Init_R_assms]:
   by simp
 
 lemma non_empty_refine_arch_state_relation[Init_R_assms]:
-  "(zeroed_arch_abstract_state, zeroed_arch_intermediate_state) \<in> arch_state_relation"
+  "(zeroed_arch_abstract_state, zeroed_arch_intermediate_state) \<in> arch_state_relation Map.empty"
   unfolding zeroed_arch_abstract_state_def zeroed_arch_intermediate_state_def arch_state_relation_def
   by (simp add: cr3_relation_def x64_irq_relation_def comp_def)
 
